wip

src/Thread.v
@@ -3,10 +3,12 @@ From Coq Require Import
      NArith.NArith
      Lists.List
      Lists.ListSet
-     (* Strings.String *)
+     Strings.String
      Morphisms
      Setoid
      RelationClasses .
+
+Import ListNotations.
 
 From ExtLib Require Import
      Structures.Monads
@@ -14,6 +16,7 @@ From ExtLib Require Import
 (*      Data.String *)
 (*      Structures.Traversable *)
 (*      Data.List. *)
+(* Import ListMonad. *)
 
 From ITree Require Import
      ITree
@@ -21,6 +24,9 @@ From ITree Require Import
      Events.Exception
      Events.Nondeterminism
      Events.State.
+Import Monads.
+Import MonadNotation.
+Import ITreeNotations.
 
 (* The [sum1] types with automatic application of commutativity and
    associativity are prone to infinite instance resolution loops.
@@ -28,12 +34,7 @@ From ITree Require Import
 Typeclasses eauto := 5.
 
 From RecordUpdate Require Import RecordSet.
-
-Import ListMonad.
-Import ITreeNotations.
-Import Monads.
-Import MonadNotation.
-Import ListNotations.
+Import RecordSetNotations.
 
 Require Import
         Types
@@ -42,114 +43,152 @@ Require Import
 Local Open Scope list.
 Local Open Scope itree_scope.
 Local Open Scope monad_scope.
-(* Local Open Scope monad_scope. *)
+Local Open Scope record_set.
 
 Definition instruction_id_t := id_t.
+Definition mem_read_id_t := id_t.
+Definition mem_write_id_t := id_t.
 
 Module Denote (Arc : ArcSig).
-  Definition mem_read_id_t := id_t.
-  Record mem_read : Type :=
-    mk_mem_read { read_id : mem_read_id_t;
-                  read_fp : Arc.mem_slc;
-                  read_kind : Arc.InsSem.mem_read_kind }.
-
-  Definition mem_write_id_t := id_t.
-  Record mem_write : Type :=
-    mk_mem_write { write_id : mem_write_id_t;
-                   write_fp : Arc.mem_slc;
-                   write_kind : Arc.InsSem.mem_read_kind }.
-
-
-  Variant storageE : Type -> Type :=
-
   Variant threadE : Type -> Type :=
-  | ThEInsFetch : Arc.InsSem.pc_t -> threadE Arc.InsSem.machine_code
-  | ThEInsDecode : Arc.InsSem.machine_code -> threadE Arc.InsSem.ast
-  | ThEInsNextLocs : Arc.InsSem.pc_t -> Arc.InsSem.ast ->
-                     threadE (list (instruction_id_t * Arc.InsSem.pc_t))
-  | ThEInsFinish : threadE unit
-  (* Load instruction *)
-  | ThEInsInitReads : Arc.mem_slc -> threadE (list mem_read_id_t)
-  | ThEInsWriteForward : mem_read_id_t -> threadE bool
-  | ThEInsReadFromSto : mem_read_id_t -> threadE bool
-  | ThEGetValueOfReads : threadE Arc.mem_slc_val.
-  (* | ThEInsSem : forall A, Arc.InsSem.E A -> threadE (option A). *)
-  (* Arguments ThEInsSem {A}. *)
+  | ThEInsFetchAndDecode : threadE Arc.InsSem.ast
+  | ThEInsNextLocs : threadE (list instruction_id_t)
+  | ThEFinishIns : threadE unit
+  | ThERegAccess : forall A, Arc.InsSem.regE A -> threadE A
+  (** Load events *)
+  | ThEInitMemLoadOps : Arc.mem_slc -> threadE (list mem_read_id_t)
+  (* [ThESatMemLoadOpForwarding] returns a bool that indicates if the read
+     was fully satisfied, and a list of iids that should be restarted. *)
+  | ThESatMemLoadOpForwarding : mem_read_id_t -> threadE (bool * list mem_write_id_t)
+  (* [ThESatMemLoadOpStorage] returns a list of iids that should be restarted. *)
+  | ThESatMemLoadOpStorage : mem_read_id_t -> threadE (list mem_write_id_t)
+  | ThECompleteLoadOps : threadE Arc.mem_slc_val
+  (** Store events *)
+  | ThEInitMemStoreOpFps : Arc.mem_slc -> threadE unit
+  | ThEInstaMemStoreOpVals : Arc.mem_slc_val -> threadE unit
+  | ThECommitStoreInstruction : threadE (list mem_write_id_t)
+  (* [ThEPropagateStoreOp] returns a list of iids that should be restarted. *)
+  | ThEPropagateStoreOp : mem_write_id_t -> threadE (list instruction_id_t)
+  | ThECompleteStoreOps : threadE unit.
 
-  Definition handle_regE {E} `{threadE -< E} `{nondetFinE -< E}
+  Definition lift_regE {E} `{threadE -< E}
     : Arc.InsSem.regE ~> itree E :=
-    fun _ e =>
-      match e with
-      | Arc.InsSem.RegERead rslc => ITree.spin (* FIXME: *)
-      | Arc.InsSem.RegEWrite rslc rval => ITree.spin (* FIXME: *)
-      end.
+    fun _ e => trigger (ThERegAccess _ e).
 
-  Definition handle_mem_read {E} `{threadE -< E} `{nondetFinE -< E}
-             (slc : Arc.mem_slc) : itree E Arc.mem_slc_val :=
-    rids <- trigger (ThEInsInitReads slc)
-    ;; ITree.iter (fun rids (* rids that aren't fully satisfied yet *) =>
+  Definition denote_restarts {E} `{schedulerE instruction_id_t -< E}
+    : ktree E (list instruction_id_t) unit :=
+    ITree.iter (fun restarts =>
+                  match restarts with
+                  | [] => ret (inr tt)
+                  | riid::restarts =>
+                    trigger (Kill riid)
+                    ;; trigger (Spawn riid)
+                    ;; ret (inl restarts)
+                  end).
+
+  Definition lift_mem_read {E}
+             `{threadE -< E} `{nondetFinE -< E}
+             `{schedulerE instruction_id_t -< E}
+             (slc : Arc.mem_slc)
+    : itree E Arc.mem_slc_val :=
+    rids <- trigger (ThEInitMemLoadOps slc)
+    ;; ITree.iter (fun rids => (* Reads that aren't fully satisfied yet. *)
                      match rids with
-                     | [] => (* All the reads are satisfied *)
-                       v <- trigger ThEGetValueOfReads
+                     | [] =>
+                       v <- trigger ThECompleteLoadOps
                        ;; ret (inr v)
                      | _ =>
                        rid <- choose rids
-                       ;; read_event <- choose [ThEInsWriteForward rid;
-                                              ThEInsReadFromSto rid]
-                       ;; is_sat <- trigger read_event
-                       ;; ret (inl (if (is_sat : bool) then List.remove Nat.eq_dec rid rids else rids))
+                       ;; read <- choose [trigger (ThESatMemLoadOpForwarding rid);
+                                        (restarts <- trigger (ThESatMemLoadOpStorage rid)
+                                         ;; ret (true, restarts))]
+                       ;; '(is_sat, restarts) <- read
+                       ;; 'tt <- denote_restarts restarts
+                       ;; ret (inl (if (is_sat : bool) then
+                                      List.remove Nat.eq_dec rid rids
+                                    else rids))
                      end) rids.
 
-  Definition handle_memE {E} `{threadE -< E} `{nondetFinE -< E}
+  Definition lift_mem_write_fp {E} `{threadE -< E} `{nondetFinE -< E}
+             (slc : Arc.mem_slc)
+    : itree E unit :=
+    trigger (ThEInitMemStoreOpFps slc).
+
+  Definition lift_mem_write_val {E}
+             `{threadE -< E} `{nondetFinE -< E}
+             `{schedulerE instruction_id_t -< E}
+             (val : Arc.mem_slc_val)
+    : itree E unit :=
+    'tt <- trigger (ThEInstaMemStoreOpVals val)
+    ;; wids <- trigger ThECommitStoreInstruction
+    ;; ITree.iter (fun wids => (* wids that haven't been propagated yet *)
+                     match wids with
+                     | [] =>
+                       'tt <- trigger ThECompleteStoreOps
+                       ;; ret (inr tt)
+                     | _ =>
+                       wid <- choose wids
+                       ;; restarts <- trigger (ThEPropagateStoreOp wid)
+                       ;; 'tt <- denote_restarts restarts
+                       ;; ret (inl (List.remove Nat.eq_dec wid wids))
+                     end) wids.
+
+  Definition lift_memE {E}
+             `{threadE -< E} `{nondetFinE -< E}
+             `{schedulerE instruction_id_t -< E}
     : Arc.InsSem.memE ~> itree E :=
     fun _ e =>
       match e with
       | Arc.InsSem.MemERead loc => (* FIXME: InsSem should use slc instead of loc *)
-        handle_mem_read {| Arc.location := loc;
-                           Arc.size := 1 |}
-      | Arc.InsSem.MemEWrite loc val => ITree.spin (* FIXME: *)
+        lift_mem_read {| Arc.location := loc;
+                         Arc.size := 1 |}
+      | Arc.InsSem.MemEWriteFP loc => (* FIXME: InsSem should use slc instead of loc *)
+        lift_mem_write_fp {| Arc.location := loc;
+                               Arc.size :=1 |}
+      | Arc.InsSem.MemEWriteVal val => lift_mem_write_val val
       end.
 
-  Definition lift_ins_sem {E} `{threadE -< E} `{nondetFinE -< E}
+  Definition lift_ins_sem {E}
+             `{threadE -< E} `{nondetFinE -< E}
+             `{schedulerE instruction_id_t -< E}
     : itree Arc.InsSem.E ~> itree E :=
     fun _ it =>
-      let h := case_ handle_regE handle_memE in
+      let h := case_ lift_regE lift_memE in
       interp h it.
 
   Definition new_instruction {E}
              `{wrapE threadE instruction_id_t -< E} `{nondetFinE -< E}
-    : ktree (schedulerE (instruction_id_t * Arc.InsSem.pc_t) +' E)
-            (instruction_id_t * Arc.InsSem.pc_t)
+    : ktree (schedulerE instruction_id_t +' E)
+            instruction_id_t
             (Types.result unit unit) :=
-    fun '(id, loc) =>
-      let it : itree (threadE +' nondetFinE +' schedulerE (instruction_id_t * Arc.InsSem.pc_t))
+    fun iid =>
+      let it : itree (threadE +' nondetFinE +' schedulerE instruction_id_t)
                      (Types.result unit unit) :=
-          mem_val <- trigger (ThEInsFetch loc)
-          ;; ast <- trigger (ThEInsDecode mem_val)
-          ;; next_ins <- trigger (ThEInsNextLocs loc ast)
-          ;; ITree.iter (fun next_ins =>
-                           match next_ins with
+          ast <- trigger ThEInsFetchAndDecode
+          ;; next_iids <- trigger ThEInsNextLocs
+          ;; ITree.iter (fun next_iids =>
+                           match next_iids with
                            | [] => ret (inr tt)
-                           | (nid, nloc)::next_ins => trigger (Spawn (nid, nloc))
-                                                    ;; ret (inl next_ins)
-                           end) next_ins
+                           | niid::next_ins => trigger (Spawn niid)
+                                            ;; ret (inl next_iids)
+                           end) next_iids
           ;; 'tt <- resum_it _ (lift_ins_sem _ (Arc.InsSem.denote ast))
-          ;; 'tt <- trigger ThEInsFinish
+          ;; 'tt <- trigger ThEFinishIns
           ;; ret (Accept tt) in
       (* Finnaly, wrap the threadE events with the iid *)
-      resum_it _ (wrap_event_in_it threadE id _ it).
+      resum_it _ (wrap_event_in_it threadE iid _ it).
 
   Definition denote {E}
              `{wrapE threadE instruction_id_t -< E} `{nondetFinE -< E}
-    : ktree E (instruction_id_t * Arc.InsSem.pc_t) (Types.result unit unit) :=
-    fun '(id, loc) =>
-      resum_it _ (scheduler new_instruction
+    : ktree E instruction_id_t (Types.result unit unit) :=
+    fun iid =>
+      resum_it _ (scheduler Nat.eq_dec new_instruction
                             (fun r1 r2 => match r1, r2 with
                                        | Accept tt, Accept tt => Accept tt
                                        | _, _ => Reject tt
                                        end)
                             (Accept tt)
-                            [new_instruction (id, loc)]).
+                            [(iid, new_instruction iid)]).
 End Denote.
 
 (*******************************************************************************)
@@ -157,160 +196,232 @@ End Denote.
 Module State(Arc : ArcSig).
   Module DenoteA := Denote Arc.
 
-  Record mem_reads :=
-    mk_mem_reads { mr_footprint : Arc.mem_slc;
-                   mr_reads : list DenoteA.mem_read;
-                   mr_unsat_slcs : DenoteA.mem_read_id_t -> option (list Arc.mem_slc);
-                   mr_reads_from :
-                     DenoteA.mem_read_id_t -> option (list (instruction_id_t * DenoteA.mem_write_id_t * Arc.mem_slc)) }.
+  Record mem_read : Type :=
+    mk_mem_read { read_id : mem_read_id_t;
+                  read_fp : Arc.mem_slc;
+                  read_kind : Arc.InsSem.mem_read_kind }.
 
-  Record mem_writes :=
-    mk_mem_writes { mw_footprint : Arc.mem_slc;
-                    mw_writes : list DenoteA.mem_write;
-                    mw_write_val : DenoteA.mem_write_id_t -> option Arc.mem_slc_val;
-                    mw_has_propagated : DenoteA.mem_write_id_t -> option bool;
-                    mw_committed : bool }.
+  Record mem_reads_state :=
+    mk_mem_reads_state { rs_footprint : Arc.mem_slc;
+                         rs_reads : list mem_read;
+                         rs_unsat_slcs : list (list Arc.mem_slc);
+                         rs_reads_from : list (list (instruction_id_t * mem_write_id_t * Arc.mem_slc)) }.
 
-  Variant instruction_exec_state : Type :=
-  (* | IESInitial : instruction_exec_state *)
-  | IESFetched : instruction_exec_state
-  | IESInstSem : instruction_exec_state
-  | IESMemRead : instruction_exec_state
-  | IESMemWrite : instruction_exec_state.
+  Record mem_write : Type :=
+    mk_mem_write { write_id : mem_write_id_t;
+                   write_fp : Arc.mem_slc;
+                   write_val : Arc.mem_slc_val;
+                   write_kind : Arc.InsSem.mem_read_kind }.
+
+  Record mem_writes_state :=
+    mk_mem_writes_state { ws_fps : list Arc.mem_slc;
+                          ws_writes : list mem_write;
+                          ws_has_propagated : list bool }.
+
+  Record reg_read_state :=
+    mk_reg_read_state { rrs_slc : Arc.InsSem.reg_slc;
+                        rrs_feeding_addr : bool;
+                        rrs_read_from : list (instruction_id_t * nat)
+                                             (* the [nat] is an index into [ins_reg_writes.rws_slc]
+                                                of the instruction pointed by the [instruction_id_t]. *)
+                        rrs_val : option Arc.InsSem.reg_val }.
+
+  Record reg_write_state :=
+    mk_reg_write_state { rws_slc : Arc.InsSem.reg_slc;
+                         rws_val : option Arc.InsSem.reg_val;
+                         (* [rws_deps] is a concatination of all the
+                            [rrs_read_from] of the instruction, when the
+                            reg-write was performed. We assume that there is a
+                            dataflow from those to this reg-write, and therefore
+                            a dependency between the feeding instructions and
+                            any instruction that reads from this
+                            register-write. *)
+                         rws_deps : list (instruction_id_t * nat);
+                         rws_load_dep : bool }.
 
   Record decoded_instruction_state :=
     mk_decoded_instruction_state {
-        ins_id : instruction_id_t;
-        ins_loc : Arc.mem_loc; (*: record fetched address :*)
         (* statically analysed data about the instruction*)
         ins_kind: Arc.instruction_kind;
 
-        (*: The input registers, for ease of dependency calculation :*)
-        ins_regs_in : ListSet.set Arc.InsSem.reg_slc;
+        ins_reg_reads : list reg_reads_state;
+        ins_reg_writes : list reg_writes_state;
 
-        (*: The input registers that feed into a memory access address :*)
-        ins_regs_feeding_address: ListSet.set Arc.InsSem.reg_slc;
-        (*: The output registers, for ease of dependency calculation *)
-        ins_regs_out: ListSet.set Arc.InsSem.reg_slc;
+        reg_writes: list (Arc.InsSem.reg_ * (list register_write_dependency * register_value));
 
-        (* dynamic info *)
+        ins_mem_reads: option mem_reads_state;
+        ins_mem_writes: option mem_writes_state;
 
-        (* reg_reads: list (reg * register_read_sources * reg_val); *)
-
-        (* reg_writes: list (reg_name * (list register_write_dependency * register_value)); *)
-
-        ins_mem_reads: option mem_reads;
-        ins_mem_writes: option mem_writes;
-
-        ins_finished: bool;
-
-        ins_exec_state: instruction_exec_state }.
+        ins_finished: bool }.
 
   Instance eta_decoded_instruction_state : Settable _ :=
-    settable! mk_decoded_instruction_state <ins_id; ins_loc; ins_kind; ins_regs_in; ins_regs_feeding_address; ins_regs_out; ins_mem_reads; ins_mem_writes; ins_finished; ins_exec_state>.
+    settable! mk_decoded_instruction_state <ins_kind; ins_regs_in; ins_regs_feeding_address; ins_regs_out; ins_mem_reads; ins_mem_writes; ins_finished>.
 
-  Definition initial_decoded_instruction_state (loc : Arc.mem_loc)
+  Definition initial_decoded_instruction_state
              (ast : Arc.InsSem.ast)
     : decoded_instruction_state :=
     let '(regs_in, regs_feeding_address, regs_out) := Arc.InsSem.regs_from_ast ast in
     (* instruction_state: *)
-    {| ins_id := 0; (* FIXME: get fresh id *)
-       ins_loc := loc;
-       ins_kind := (Arc.instruction_kind_from_ast ast);
+    {| ins_kind := (Arc.instruction_kind_from_ast ast);
        ins_regs_in := regs_in;
        ins_regs_feeding_address := regs_feeding_address;
        ins_regs_out := regs_out;
        ins_mem_reads := None;
        ins_mem_writes := None;
-       ins_finished := false;
-       ins_exec_state := IESFetched |}.
+       ins_finished := false |}.
 
-  Variant instruction_state :=
-  | ISUnfetched : Arc.mem_loc -> instruction_state
-  | ISFetched : Arc.mem_loc -> Arc.InsSem.machine_code -> instruction_state
-  | ISDecoded : decoded_instruction_state -> instruction_state.
+  Definition instruction_state : Type := instruction_id_t *
+                                         Arc.mem_loc *
+                                         option decoded_instruction_state.
 
   Record state :=
-    mk_state {
-        next_iid : instruction_id_t;
-        instruction_tree : tree instruction_state }.
+    mk_state { next_iid : instruction_id_t;
+               instruction_tree : tree instruction_state }.
 
   Instance eta_state : Settable _ :=
     settable! mk_state <next_iid; instruction_tree>.
 
   Definition initial_state (loc : Arc.mem_loc)
     : state :=
-    {| next_iid := 0;
-       instruction_tree := Tree (ISUnfetched loc) [] |}.
+    {| next_iid := 1;
+       instruction_tree := Tree (0, loc, None) [] |}.
 
-  Definition read_reg_slc (rslc : Arc.InsSem.reg_slc) (iid : instruction_id_t) (s : state)
-    : (state * Arc.InsSem.reg_val) :=
-    (* FIXME: *)
-    (s, 0%N).
+  Variant storageE : Type -> Type :=
+  | StEReadInstruction : Arc.InsSem.pc_t -> storageE Arc.InsSem.machine_code
+  | StERead : mem_read_id_t -> storageE unit.
 
-  Definition write_reg_slc (rslc : Arc.InsSem.reg_slc) (val : Arc.InsSem.reg_val)
+  Definition get_instruction_state {E} `{exceptE error -< E}
              (iid : instruction_id_t) (s : state)
+    : itree E instruction_state :=
+    let fix helper t :=
+        let '(Tree ((iid', _, _) as i) ts) := t in
+        if Nat.eqb iid' iid then Some i
+        else
+          match List.find (fun x => match x with None => false | _ => true end)
+                          (List.map helper ts) with
+          | Some x => x
+          | None => None
+          end
+    in
+    try_unwrap_option (helper s.(instruction_tree)) "get_instruction_state: Can't find iid".
+
+  Definition get_dec_instruction_state {E} `{exceptE error -< E}
+             (iid : instruction_id_t) (s : state)
+    : itree E decoded_instruction_state :=
+    '(_, _, ins) <- get_instruction_state iid s
+    ;; try_unwrap_option ins "get_dec_instruction_state: instruction was not decoded yet".
+
+  Definition update_dec_instruction_state (iid : instruction_id_t)
+             (ins : decoded_instruction_state) (s : state)
     : state :=
-    (* FIXME: *)
-    s.
+    let fix helper t :=
+        let '(Tree ((iid', loc, _) as i) ts) := t in
+        if Nat.eqb iid' iid then Tree (iid, loc, Some ins) ts
+        else Tree i (List.map helper ts)
+    in
+    s <| instruction_tree := helper s.(instruction_tree) |>.
 
+  Definition try_read_reg_slc {E}
+             (rslc : Arc.InsSem.reg_slc) (iid : instruction_id_t) (s : state)
+    : itree E (state * Arc.InsSem.reg_val) :=
+    ITree.spin.
 
-  Definition handle_regE {E} : wrapE Arc.InsSem.regE instruction_id_t ~> stateT state (itree E) :=
-    fun _ e s =>
-      let '(Wrap e iid) := e in
-      match e with
-      | Arc.InsSem.RegERead rslc => Ret (read_reg_slc rslc iid s)
-      | Arc.InsSem.RegEWrite rslc rval => Ret (write_reg_slc rslc rval iid s, tt)
-      end.
+  Definition try_write_reg_slc {E}
+             (rslc : Arc.InsSem.reg_slc) (val : Arc.InsSem.reg_val)
+             (iid : instruction_id_t) (s : state)
+    : itree E (state * unit) :=
+    ins <- get_dec_instruction_state iid s
+    ;; update_dec_instruction_state iid () s
 
-  Definition handle_threadE {E}
+  Definition handle_reg_access {E} `{exceptE error -< E}
+             {A} (e : Arc.InsSem.regE A) (iid : instruction_id_t) (s : state)
+    : itree E (state * A) :=
+    match e with
+    | Arc.InsSem.RegERead rslc => try_read_reg_slc rslc iid s
+    | Arc.InsSem.RegEWrite rslc rval => try_write_reg_slc rslc rval iid s
+    end.
+
+  Definition try_fetch_and_decode {E} `{storageE -< E} `{exceptE error -< E}
+             (iid : instruction_id_t) (s : state)
+    : itree E (state * Arc.InsSem.ast) :=
+    '(_, loc, _) <- get_instruction_state iid s
+    ;; mem_read_result <- trigger (StEReadInstruction loc)
+    ;; code <- value_from_mem_read_result mem_read_result
+    ;; ast <- Arc.InsSem.decode code
+    ;; let ins := initial_decoded_instruction_state ast in
+       let s := update_dec_instruction_state iid ins s in
+       ret (s, ast).
+
+  Definition try_get_next_locations {E} `{exceptE error -< E}
+             (iid : instruction_id_t) (s : state)
+    : itree E (state * list instruction_id_t) :=
+    iic <- get_instruction_in_context iid s
+    ;; ins <- get_decoded_instruction_state iic
+    ;; let next_pcs := Arc.InsSem.next_pc ins.(ins_loc) ins.(ins_ast) in
+       let iids := List.seq s.(next_iid) (List.length next_pcs) in
+       let iidpcs := List.combine iids next_pcs in
+       let new_subtrees := List.map (fun (iid, pc) => Tree (ISUnfetched pc) []) iidpcs in
+       let s := s <| next_iid := s.(next_iid) + (List.length next_pcs) |>
+                  <| instruction_tree := apply_tree_context iic.(iic_context) iic.(iic_instruction) new_subtrees |> in
+       ret (s, iids).
+
+  Definition try_init_mem_load_ops {E} `{exceptE error -< E}
+             (slc : Arc.mem_slc) (iid : instruction_id_t) (s : state)
+    : itree E (state * list mem_read_id_t) :=
+    throw NotImplemented.
+
+  Definition try_write_forward {E} `{exceptE error -< E}
+             (rid : mem_read_id_t) (iid : instruction_id_t) (s : state)
+    : itree E (state * bool) :=
+    throw NotImplemented.
+
+  Definition try_sat_mem_load_op_from_storage {E} `{storageE -< E} `{exceptE error -< E}
+             (rid : mem_read_id_t) (iid : instruction_id_t) (s : state)
+    : itree E (state * unit) :=
+    iic <- get_instruction_in_context iid s
+    ;; ins <- get_decoded_instruction_state iic
+    ;; rr <- get_mem_read_request rid ins
+    ;; mem_read_result <- trigger (StoERead rr)
+    ;; ins <- update_mem_read_request mem_read_result rid ins
+    ;; let s := <| instruction_tree := apply_tree_context iic.(iic_context) (ISDecoded ins) iic.(iic_subtrees) |> in
+       ret (s, tt).
+
+  Definition try_complete_load_ops {E} `{exceptE error -< E}
+             (iid : instruction_id_t) (s : state)
+    : itree E (state * mem_slc_val) :=
+    iic <- get_instruction_in_context iid s
+    ;; ins <- get_decoded_instruction_state iic
+    ;; val <- get_mem_reads_value ins
+    ;; ret (s, val).
+
+  Definition try_finish_instruction {E} `{exceptE error -< E}
+             (iid : instruction_id_t) (s : state)
+    : itree E (state * unit) :=
+    throw NotImplemented.
+
+  Definition handle_threadE {E} `{storageE -< E} `{exceptE error -< E}
     : wrapE ThrDenote.threadE Thread.instruction_id_t ~>
             stateT state (itree E) :=
     fun _ e s =>
       let '(Wrap e iid) := e in
       match e with
-      | ThEInsFetch _ => ITree.spin
-      | ThEInsReadFromSto _ => ITree.spin
-
-      | ThEInsDecode code =>
-        match Arc.InsSem.decode code with
-        | Some ast =>
-          (* FIXME: update [s] *)
-          Ret (s, ast)
-        | None => throw InsDecodeFail
-        end
-
-      | ThEInsNextLocs loc ast =>
-        let next_pcs := Arc.InsSem.next_pc loc ast in
-        let iids := List.seq s.(next_iid) (List.length next_pcs) in
-        let s := s <| next_iid := s.(next_iid) + (List.length next_pcs) |> in
-        Ret (s, list.compose iids next_pcs)
-
-      | ThEInsDecode : Arc.InsSem.machine_code -> threadE Arc.InsSem.ast
-      | ThEInsNextLocs : Arc.InsSem.pc_t -> Arc.InsSem.ast ->
-                         threadE (list (instruction_id_t * Arc.InsSem.pc_t))
-      | ThEInsFinish : threadE unit
-      (* Load instruction *)
-      | ThEInsInitReads : Arc.mem_slc -> threadE (list mem_read_id_t)
-      | ThEInsWriteForward : mem_read_id_t -> threadE bool
-      | ThEGetValueOfReads : threadE Arc.mem_slc_val.
-
+      | ThEInsFetchAndDecode => try_fetch_and_decode iid s
+      | ThEInsNextLocs => try_get_next_locations iid s
+      | ThEFinishIns => try_finish_instruction iid s
+      | ThERegAccess _ e => handle_reg_access e iid s
+      (* Load events *)
+      | ThEInitMemLoadOps slc => try_init_mem_load_ops slc iid s
+      | ThESatMemLoadOpForwarding rid => throw NotImplemented
+      | ThESatMemLoadOpStorage rid => try_sat_mem_load_op_from_storage rid iid s
+      | ThECompleteLoadOps => try_complete_load_ops iid s
+      (* Store events *)
+      (* | ThEInitMemStoreOpFps : Arc.mem_slc -> threadE unit *)
+      (* | ThEInstaMemStoreOpVals : Arc.mem_slc_val -> threadE unit *)
+      (* | ThECommitStoreInstruction : threadE (list mem_write_id_t) *)
+      (* | ThEPropagateStoreOp : mem_write_id_t -> threadE unit *)
+      (* | ThECompleteStoreOps : threadE unit. *)
       end.
 
-  (* Definition handle_thread {E} : Arc.InsSem.E ~> stateT thread_state (itree E) :=. *)
-
-  (* Definition handle_thread {E} : threadE ~> stateT thread_state (itree E) := *)
-  (*   fun _ e thread_state => *)
-  (*     match e with *)
-  (*     | *)
-
-  (* (* SAZ: I think that all of these [run_foo] functions should be renamed *)
-  (*    [interp_foo].  That would be more consistent with the idea that *)
-  (*    we define semantics by nested interpretation.  Also, it seems a bit *)
-  (*    strange to define [interp_map] in terms of [interp_state]. *)
-  (* *) *)
-  (* Definition interp_map {E d} : itree (mapE d +' E) ~> stateT map (itree E) := *)
-  (*   interp_state (case_ handle_map pure_state). *)
 
 
 End State.
